basic_return.thy
@@ -89,6 +89,7 @@ lemma first_chars_return:
 lemma b_return_well_formed:
   "bidef_well_formed (return v)"
   apply wf_init
+  subgoal by (rule return_PNGI)
   subgoal by (simp add: parser_can_parse_print_result_def
                         return_def fp_NER NER_simps)
   subgoal by (simp add: printer_can_print_parse_result_def
